src/sequential/SequentialBehavior.v
@@ -28,6 +28,18 @@ Proof.
   ii. destruct x, y, z; ss. etrans; eauto.
 Qed.
 
+Program Instance Forall2_PreOrder A R `{@PreOrder A R}: PreOrder (Forall2 R).
+Next Obligation.
+Proof.
+  ii. induction x; econs; auto. refl.
+Qed.
+Next Obligation.
+Proof.
+  intros x. induction x.
+  { ii. inv H0; inv H1. econs. }
+  { ii. inv H0; inv H1. econs; eauto. etrans; eauto. }
+Qed.
+
 
 Module SeqEvent.
   Variant t: Set :=
@@ -46,8 +58,42 @@ Module SeqEvent.
   | syscall
       (e: Event.t)
       (d: diffs) (f: Flags.t) (m_released: SeqMemory.t)
-  | failure
   .
+
+  Definition get_event (e: ProgramEvent.t) (m: SeqMemory.t) (d: diffs) (m_released: option SeqMemory.t): option t :=
+    match e with
+    | ProgramEvent.silent | ProgramEvent.failure => None
+    | ProgramEvent.read loc val ord =>
+      let f := if Ordering.le Ordering.acqrel ord
+               then (Some (SeqMemory.flags m)) else None in
+      Some (read loc val ord d (m loc) f)
+    | ProgramEvent.write loc val ord =>
+      let m_released := if Ordering.le Ordering.strong_relaxed ord
+                        then m_released
+                        else None in
+      Some (write loc val ord d (m loc) m_released)
+    | ProgramEvent.update loc valr valw ordr ordw =>
+      let f := if Ordering.le Ordering.acqrel ordr
+               then (Some (SeqMemory.flags m)) else None in
+      let m_released := if Ordering.le Ordering.strong_relaxed ordw
+                        then m_released
+                        else None in
+      Some (update loc valr valw ordr ordw d (m loc) f m_released)
+    | ProgramEvent.fence ordr ordw =>
+      let f := if Ordering.le Ordering.acqrel ordr
+               then (Some (SeqMemory.flags m)) else None in
+      let m_released := if Ordering.le Ordering.strong_relaxed ordw
+                        then m_released
+                        else None in
+      Some (fence ordr ordw d f m_released)
+    | ProgramEvent.syscall e =>
+      let f := (SeqMemory.flags m) in
+      match m_released with
+      | None => None
+      | Some m_released =>
+        Some (syscall e d f m_released)
+      end
+    end.
 
   Variant le: t -> t -> Prop :=
   | le_read
@@ -81,9 +127,6 @@ Module SeqEvent.
       (RELEASED: SeqMemory.le m0 m1)
     :
       le (syscall e d f0 m0) (syscall e d f1 m1)
-  | le_failure
-    :
-      le failure failure
   .
 
   Program Instance le_PreOrder: PreOrder le.
@@ -105,46 +148,183 @@ Module SeqTrace.
   | ub (es: list SeqEvent.t)
   .
 
+  Definition cons (e: SeqEvent.t) (tr: t): t :=
+    match tr with
+    | term es m => term (e::es) m
+    | partial es f => partial (e::es) f
+    | ub es => ub (e::es)
+    end.
+
+  Definition cons_opt (e: option SeqEvent.t) (tr: t): t :=
+    match e with
+    | Some e => cons e tr
+    | None => tr
+    end.
+
   Variant le: t -> t -> Prop :=
   | le_term
-      es_src es_tgt m_tgt m_src
+      es_src es_tgt m_src m_tgt
       (EVENTS: Forall2 SeqEvent.le es_tgt es_src)
       (MEMORY: SeqMemory.le m_tgt m_src)
     :
       le (term es_tgt m_tgt) (term es_src m_src)
   | le_pterm
-      es0 es1 es2 m0 m1
-      (EVENTS: Forall2 SeqEvent.le es0 es1)
-      (FLAGS: Flags.le f0 f1)
+      es_src es_tgt f_src f_tgt
+      (EVENTS: exists es_hd es_tl,
+          (<<APP: es_src = es_hd ++ es_tl>>) /\
+          (<<FORALL: Forall2 SeqEvent.le es_tgt es_hd>>))
+      (FLAGS: Flags.le f_tgt f_src)
     :
-      le (pterm es0 f0) (pterm es1 f1)
+      le (partial es_tgt f_tgt) (partial es_src f_src)
+  | le_ub
+      es_src tr_tgt
+    :
+      le tr_tgt (ub es_src)
+  .
+
+  Program Instance le_PreOrder: PreOrder le.
+  Next Obligation.
+  Proof.
+    ii. destruct x.
+    { econs 1; refl. }
+    { econs 2; [|refl]. exists es, []. splits; [|refl].
+      rewrite app_nil_r. auto. }
+    { econs 3. }
+  Qed.
+  Next Obligation.
+  Proof.
+    ii. inv H; inv H0.
+    { econs 1; eauto.
+      { etrans; eauto. }
+      { etrans; eauto. }
+    }
+    { econs 3. }
+    { des; subst.
+      eapply Forall2_app_inv_l in FORALL. des; subst.
+      econs 2.
+      { eexists l1', (l2' ++ es_tl). splits.
+        { rewrite app_assoc. auto. }
+        { etrans; eauto. }
+      }
+      { etrans; eauto. }
+    }
+    { econs 3. }
+    { econs 3. }
+  Qed.
+
+  Definition incl (b0: t -> Prop) (b1: t -> Prop): Prop :=
+    forall tr0, b0 tr0 -> exists tr1, b1 tr1 /\ le tr0 tr1.
+
+  Program Instance incl_PreOrder: PreOrder incl.
+  Next Obligation.
+  Proof.
+    ii. exists tr0. split; auto. refl.
+  Qed.
+  Next Obligation.
+  Proof.
+    ii. apply H in H1. des. apply H0 in H1. des.
+    esplits; eauto. etrans; eauto.
+  Qed.
+End SeqTrace.
 
 
+Module SeqBehavior.
+Section LANG.
+  Variable lang: language.
+
+  Inductive behavior: forall (th0: SeqThread.t lang) (tr: SeqTrace.t), Prop :=
+  | behavior_term
+      st m p o
+      (TERMINAL: lang.(Language.is_terminal) st)
+    :
+      behavior (SeqThread.mk (SeqState.mk _ st m) p o) (SeqTrace.term [] m)
+  | behavior_partial
+      st m p o
+    :
+      behavior (SeqThread.mk (SeqState.mk _ st m) p o) (SeqTrace.partial [] (SeqMemory.flags m))
+  | behavior_ub
+      st m p o
+      (FAILURE: SeqThread.failure (SeqThread.mk (SeqState.mk _ st m) p o))
+    :
+      behavior (SeqThread.mk (SeqState.mk _ st m) p o) (SeqTrace.ub [])
+  | behavior_na_step
+      th0 th1 tr
+      (STEP: SeqThread.na_step MachineEvent.silent th0 th1)
+      (BEHAVIOR: behavior th1 tr)
+    :
+      behavior th0 tr
+  | behavior_at_step
+      th0 th1 pe d m_released e tr
+      (STEP: SeqThread.at_step pe d m_released th0 th1)
+      (EVENT: SeqEvent.get_event pe th0.(SeqThread.state).(SeqState.memory) d m_released = Some e)
+      (BEHAVIOR: behavior th1 tr)
+    :
+      behavior th0 (SeqTrace.cons e tr)
+  .
+End LANG.
+
+Definition refine
+           (lang_tgt lang_src: language)
+           (st_tgt: lang_tgt.(Language.state)) (st_src: lang_src.(Language.state))
+  : Prop :=
+  forall o p vals (WF: Oracle.wf o),
+    SeqTrace.incl
+      (behavior (SeqThread.mk (SeqState.mk _ st_tgt (SeqMemory.init vals)) p o))
+      (behavior (SeqThread.mk (SeqState.mk _ st_src (SeqMemory.init vals)) p o)) .
+End SeqBehavior.
 
 
+Section DETERMINISM.
+  Variable lang: language.
 
-  Variant
-
-          (f: option Flags.t)
-
-
-
-
-  Definition match_event (e: ProgramEvent.t) (m_tgt m_src: t): Prop :=
-    match e with
-    | ProgramEvent.silent => True
-    | ProgramEvent.read loc _ ord =>
-      (SeqCell.le (m_tgt loc) (m_src loc)) /\
-      (Ordering.le Ordering.acqrel ord -> le_partial m_tgt m_src)
-    | ProgramEvent.write loc _ _ =>
-      (SeqCell.le (m_tgt loc) (m_src loc))
-    | ProgramEvent.update loc _ _ ordr _ =>
-      (SeqCell.le (m_tgt loc) (m_src loc)) /\
-      (Ordering.le Ordering.acqrel ordr -> le_partial m_tgt m_src)
-    | ProgramEvent.fence ordr ordw =>
-      (ordw = Ordering.seqcst -> le m_tgt m_src) /\
-      (Ordering.le Ordering.acqrel ordr -> le_partial m_tgt m_src)
-    | ProgramEvent.syscall _ =>
-      le m_tgt m_src
-    | ProgramEvent.failure => True
+  Definition similar (e0 e1: ProgramEvent.t): Prop :=
+    e0 = e1 \/
+    match e0, e1 with
+    | ProgramEvent.read loc0 val0 ord0, ProgramEvent.write loc1 val1 ord1 =>
+      loc0 = loc1 /\ ord0 = ord1
+    | ProgramEvent.update loc0 valr0 valw0 ordr0 ordw0, ProgramEvent.update loc1 valr1 valw1 ordr1 ordw1 =>
+      loc0 = loc1 /\ ordr0 = ordr1 /\ ordw0 = ordw1 /\ (valr0 = valr1 -> valw0 = valw1)
+    | ProgramEvent.read loc0 val0 ord0, ProgramEvent.update loc1 valr1 valw1 ordr1 ordw1 =>
+      loc0 = loc1 /\ val0 <> valr1
+    | ProgramEvent.update loc0 valr0 valw0 ordr0 ordw0, ProgramEvent.read loc1 val1 ord1 =>
+      loc0 = loc1 /\ valr0 <> val1
+    | _, _ => False
     end.
+
+  Variant _deterministic (deterministic: lang.(Language.state) -> Prop) (st0: lang.(Language.state)): Prop :=
+  | deterministic_intro
+      (PRESERVE:
+         forall e st1 (STEP: lang.(Language.step) e st0 st1),
+           deterministic st1)
+      (STEP_TERMINAL:
+         forall e st1 (STEP: lang.(Language.step) e st0 st1)
+                (TERMINAL: lang.(Language.is_terminal) st0), False)
+      (STEP_STEP:
+         forall e1 st1 (STEP1: lang.(Language.step) e1 st0 st1)
+                e2 st2 (STEP2: lang.(Language.step) e2 st0 st2),
+           similar e1 e2 /\ (e1 = e2 -> st1 = st2))
+  .
+
+  Lemma deterministic_mon: monotone1 _deterministic.
+  Proof.
+    ii. inv IN. econs; eauto.
+  Qed.
+  Hint Resolve deterministic_mon: paco.
+
+  Definition deterministic := paco1 _deterministic bot1.
+End DETERMINISM.
+#[export] Hint Resolve deterministic_mon: paco.
+
+
+Section ADEQUACY.
+  Variable lang_src lang_tgt: language.
+
+  Theorem refinement_imply_simulation
+          (st_src: lang_src.(Language.state)) (st_tgt: lang_tgt.(Language.state))
+          (DETERM: deterministic _ st_src)
+          (REFINE: SeqBehavior.refine _ _ st_tgt st_src)
+    :
+      sim_seq_all _ _ (fun _ _ => True) st_src st_tgt.
+  Proof.
+  Admitted.
+End ADEQUACY.
